{
 "cells": [
  {
   "cell_type": "markdown",
   "id": "94f4431a",
   "metadata": {},
   "source": [
    "1. Find the value of T(2) for the recurrence relation T(n) = 3T(n-1) + 12n, given that T(0)=5."
   ]
  },
  {
   "cell_type": "markdown",
   "id": "ce657977",
   "metadata": {},
   "source": [
    "T(n) = 3T(n-1) + 12n\n",
    "\n",
    "T(2) = 3T(2-1) + 12*2\n",
    "     = 3T(1) + 24\n",
    "    \n",
    "Now, we have to find T(1) by recurrence relation\n",
    "\n",
    "T(n) = 3T(n-1) + 12n\n",
    "\n",
    "T(1) = 3T(1-1) + 12*1\n",
    "     = 3T(0) + 12\n",
    "     = 3*5 + 12\n",
    "     = 15 +12\n",
    "     = 27\n",
    "        \n",
    "now put value of T(1) in above euation\n",
    "\n",
    "T(2) = 3T(1) + 24\n",
    "     = 3*27 + 24\n",
    "     = 81 + 24\n",
    "     = 105\n",
    "T(2) = 105"
   ]
  },
  {
   "cell_type": "markdown",
   "id": "9023791e",
   "metadata": {},
   "source": [
    "2. Given a recurrence relation, solve it using the substitution method:\n",
    "\n",
    "a. T(n) = T(n-1) + c\n",
    "\n",
    "b. T(n) = 2T(n/2) + n\n",
    "\n",
    "c. T(n) = 2T(n/2) + c\n",
    "\n",
    "d. T(n) = T(n/2) + c"
   ]
  },
  {
   "cell_type": "markdown",
   "id": "30b9c4c1",
   "metadata": {},
   "source": [
    "T(n) = T(n-1) + c --(1)\n",
    "\n",
    "T(n-1) = T(n-1-1) + c\n",
    "T(n-1) = T(n-2) + c -- (2)\n",
    "\n",
    "T(n-2) = T(n-2-1) + c\n",
    "T(n-2) = T(n-3) + c -- (3)\n",
    "\n",
    "Now from equation (1): -\n",
    "\n",
    "T(n) = T(n-1) + c\n",
    "T(n) = T(n-2) + c + c  :Put vlaue of T(n-1) from equation 2\n",
    "T(n) = T(n-2) + 2c\n",
    "T(n) = T(n-3) + c + 2c  :Put value of T(n-2) from equation 3\n",
    "T(n) = T(n-3) + 3c\n",
    "    .\n",
    "    .\n",
    "    k times\n",
    "    .\n",
    "    .\n",
    "T(n) = T(n-k) + k*c\n",
    "\n",
    "from base condition\n",
    "n-k = 1\n",
    "k = n-1\n",
    "\n",
    "T(n) = T(1) + (n-1)c"
   ]
  },
  {
   "cell_type": "markdown",
   "id": "70d0c86c",
   "metadata": {},
   "source": [
    "b. T(n) = 2T(n/2) + n\n",
    "\n",
    "    T(n) = 2T(n/2) + n -- (1)\n",
    "    T(n/2) = 2T(n/2**2) + n/2 --(2)\n",
    "    T(n/2**2) = 2T(n/2**3) + n/2**2 --(3)\n",
    "    \n",
    "    Put value of T(n/2) from equation from 2 in equation 1:\n",
    "    \n",
    "    T(n) = 2[2T(n/2**2) + n/2] + n\n",
    "    T(n) = 2**2T(n/2**2) + 2n\n",
    "    \n",
    "    put value of T(n/2**2) from equation 2 in above equation:\n",
    "    \n",
    "    T(n) = 2**2[2T(n/2**3) + n/2**2] + 2n\n",
    "    T(n) = 2**3T(n/2**3) + 3n\n",
    "        .\n",
    "        .\n",
    "        k times\n",
    "        .\n",
    "        .\n",
    "    T(n) = 2**kT(n/2**k) + kn  --(4)\n",
    "    \n",
    "    from base condition: -\n",
    "    \n",
    "    n/2**k = 1\n",
    "    n = 2**k\n",
    "    take log both sides\n",
    "    \n",
    "    logn = klog2\n",
    "    k = log2^n\n",
    "    \n",
    "    put above value in equation 4\n",
    "    \n",
    "    T(n) = nT(1) + nlog2^n\n",
    "    T(n) = n + nlog2^n"
   ]
  },
  {
   "cell_type": "markdown",
   "id": "9425b064",
   "metadata": {},
   "source": [
    "T(n) = 2T(n/2) + c  --(1)\n",
    "\n",
    "T(n/2) = 2T(n/2^2) + c  --(2)\n",
    "\n",
    "T(n/2^2) = 2T(n/2^3) + c --(3)\n",
    "\n",
    "now from equation:-\n",
    "    \n",
    "    T(n) = 2T(n/2) + c\n",
    "    T(n) = 2[2T(n/2^2) + c] + c\n",
    "    T(n) = 2^2T(n/2^2) + 2^1c +c\n",
    "    T(n) = 2^2T(n/2^2) + 2^C + c\n",
    "    \n",
    "    T(n) = 2^2[2T(n/2^3) + c] + 2^1c + c\n",
    "    T(n) = 2^3T(n/2^3) + 2^2c + 2^1c + c\n",
    "    T(n) = 2^3T(n/2^3) + 2^2c + 2^1c + 2^0c\n",
    "        .\n",
    "        .\n",
    "        k times\n",
    "        .\n",
    "        .\n",
    "    T(n) = 2^kT(n/2^k) + 2^(k-1)c + 2^(k-2)c + ..... + 2^0c -- (4)\n",
    "    \n",
    "    from base condition: -\n",
    "     n/2^k = 1\n",
    "     n = 2^k\n",
    "     take log both sides\n",
    "     k = log2^n\n",
    "     \n",
    "     keep above value in equation 4:-\n",
    "     \n",
    "     T(n) = nT(1) + 2^(log2^n -1)c + 2^(log2^n-2)c + .. +2^0c\n",
    "     T(n) = n + nlog2^n"
   ]
  },
  {
   "cell_type": "markdown",
   "id": "faa89e61",
   "metadata": {},
   "source": [
    "T(n) = T(n/2) + c --(1)\n",
    "\n",
    "T(n/2) = T(n/2^2) + c --(2)\n",
    "T(n/2^2) = T(n/2^3) + c --(3)\n",
    "\n",
    "keep value of T(n/2) and T(n/n^2) from equation from 2 and 3 in equation 1\n",
    "\n",
    "T(n) = T(n/2^2) + c + c\n",
    "\n",
    "T(n) = T(n/2^3) + c + c + c\n",
    "    .\n",
    "    .\n",
    "    k times\n",
    "T(n) = T(n/2^k) + kc\n",
    "\n",
    "from base condition\n",
    "\n",
    "    n/2^k = 1\n",
    "    n = 2^k\n",
    "    take log both sides\n",
    "    k = log2^n\n",
    "    \n",
    " T(n) = T(1) + clog2^n\n",
    " T(n) = 1 + clog2^n\n"
   ]
  },
  {
   "cell_type": "markdown",
   "id": "c9855e60",
   "metadata": {},
   "source": [
    "3. Given a recurrence relation, solve it using the recursive tree approach:\n",
    "a. T(n) = 2T(n-1) +1\n",
    "b. T(n) = 2T(n/2) + n"
   ]
  },
  {
   "cell_type": "markdown",
   "id": "ad8d06f0",
   "metadata": {},
   "source": [
    "T(n) = 2T(n-1) +1 b"
   ]
  },
  {
   "cell_type": "markdown",
   "id": "e43a109a",
   "metadata": {},
   "source": [
    "                                        2T(n-1) - 1\n",
    "                                       !        !\n",
    "                                       n-1      n-1 - 2\n",
    "                                      !   !    !   !\n",
    "                                     n-2  n-2  n-2  n-2 - 4\n",
    "                                     \n",
    "                                             .\n",
    "                                             .\n",
    "                                             k times\n",
    "                                             .\n",
    "                                             .\n",
    "base condition: -\n",
    "\n",
    "n-k = 0\n",
    "n = k\n",
    "\n",
    "\n",
    "= 2^0 + 2^1 + 2^2 + .....+ 2^n\n",
    "\n",
    "\n",
    "= 2^0(2^n-1)/(2-1)\n",
    "= 1(2^n-1)\n",
    "= 2^n -1"
   ]
  },
  {
   "cell_type": "markdown",
   "id": "12e6078a",
   "metadata": {},
   "source": [
    "T(n) = 2T(n/2) + n\n",
    "\n",
    "                    T(n)\n",
    "                 !            !\n",
    "              T(n/2)        T(n/2)\n",
    "           !         !    !       !\n",
    "         T(n/4)  T(n/4)  T(n/4)   T(n/4)\n",
    "         \n",
    "         \n",
    "In general, for each level i, there are 2^i nodes, and each node has a cost of n/2^i\n",
    "\n",
    "The total cost at each level is 2^i * n/2^i = n\n",
    "\n",
    "Now there are log2n levels in three.\n",
    "\n",
    "\n",
    "T(n) = n * log2n\n",
    "\n",
    "T(n) = nlog2n\n"
   ]
  }
 ],
 "metadata": {
  "kernelspec": {
   "display_name": "Python 3",
   "language": "python",
   "name": "python3"
  },
  "language_info": {
   "codemirror_mode": {
    "name": "ipython",
    "version": 3
   },
   "file_extension": ".py",
   "mimetype": "text/x-python",
   "name": "python",
   "nbconvert_exporter": "python",
   "pygments_lexer": "ipython3",
   "version": "3.8.8"
  }
 },
 "nbformat": 4,
 "nbformat_minor": 5
}
